A2_lists.v
@@ -78,3 +78,4 @@ End Well_founded_induction.
 End Lists.
 
 Global Hint Resolve incl_nil_l incl_cons incl_app firstn_incl skipn_incl : incl.
+Hint Rewrite firstn_length skipn_length : list.
